Frame-preserving update for first field of struct

examples/steel/ProductPCM.fst
@@ -2,6 +2,73 @@ module ProductPCM
 
 open FStar.PCM
 
+/// Aseem's alternative definition of frame-preserving updates
+
+type frame_preserving_upd (#a:Type u#a) (p:pcm a) (x y:a) =
+  v:a{
+     p.refine v /\
+     compatible p x v
+  } ->
+  v_new:a{
+    p.refine v_new /\
+    compatible p y v_new /\
+    (forall (frame:a{composable p x frame}).{:pattern composable p x frame}
+       composable p y frame /\
+       (op p x frame == v ==> op p y frame == v_new))}
+
+/// The alternative definition satisfies 3 nice properties:
+
+(* The identity function is a frame-preserving update *)
+val no_op_is_frame_preserving :
+  p: pcm 'a -> x: 'a ->
+  frame_preserving_upd p x x
+let no_op_is_frame_preserving p x = fun v -> v
+
+(* Frame-preserving updates compose, and the composition is just
+   function composition *)
+val frame_preserving_updates_compose :
+  p: pcm 'a -> x: 'a -> y: 'a -> z: 'a ->
+  frame_preserving_upd p y z ->
+  frame_preserving_upd p x y ->
+  frame_preserving_upd p x z
+let frame_preserving_updates_compose p x y z f g = fun v -> f (g v)
+
+val compatible_subframe :
+  p: pcm 'a -> x: 'a -> y: 'a {composable p x y} -> z: 'a ->
+  Lemma (requires (compatible p (op p x y) z)) (ensures (compatible p x z))
+let compatible_subframe p x y z =
+  compatible_elim p (op p x y) z (compatible p x z) (fun frame ->
+    p.comm x y;
+    p.assoc frame y x)
+
+(* A frame-preserving update from x to y is also a frame-preserving
+   update from (x `op` subframe) to (y `op` subframe), for any subframe *)
+open FStar.Classical
+val frame_preserving_subframe : 
+  p: pcm 'a -> x: 'a -> y: 'a -> subframe: 'a{composable p x subframe /\ composable p y subframe} ->
+  frame_preserving_upd p x y ->
+  frame_preserving_upd p (op p x subframe) (op p y subframe)
+let frame_preserving_subframe #a p x y subframe f v =
+  compatible_subframe p x subframe v;
+  let w = f v in
+  let aux (frame: a{composable p (op p x subframe) frame}):
+    Lemma (composable p (op p y subframe) frame /\
+           (op p (op p x subframe) frame == v ==> op p (op p y subframe) frame == w))
+           [SMTPat (composable p (op p y subframe) frame)]
+  = p.assoc_r x subframe frame;
+    assert (composable p x (op p subframe frame));
+    assert (composable p y (op p subframe frame));
+    p.assoc y subframe frame
+  in
+  let lframe : squash (compatible p (op p x subframe) v) = () in
+  exists_elim (compatible p (op p y subframe) w) lframe (fun frame -> 
+    aux frame;
+    assert (op p frame (op p x subframe) == v);
+    p.comm frame (op p x subframe);
+    assert (op p (op p y subframe) frame == w);
+    p.comm (op p y subframe) frame);
+  w
+
 /// We can define a PCM for structs with two fields {a; b} by defining
 /// a PCM for tuples (a & b) in terms of (potentially user-defined)
 /// PCMs for a and b.
@@ -12,21 +79,169 @@ let tuple_comp p q (xa, xb) (ya, yb) = composable p xa ya /\ composable q xb yb
 val tuple_op : p: pcm 'a -> q: pcm 'b -> x:('a & 'b) -> y:('a & 'b){tuple_comp p q x y} -> 'a & 'b
 let tuple_op p q (xa, xb) (ya, yb) = (op p xa ya, op q xb yb)
 
-val tuple_pcm : pcm 'a -> pcm 'b -> pcm ('a & 'b)
-let tuple_pcm p q = FStar.PCM.({
-  p = {
-    composable=tuple_comp p q;
-    op=tuple_op p q;
-    one=(p.p.one, q.p.one)
-  };
-  comm = (fun (xa, xb) (ya, yb) -> p.comm xa ya; q.comm xb yb);
-  assoc = (fun (xa, xb) (ya, yb) (za, zb) -> p.assoc xa ya za; q.assoc xb yb zb);
-  assoc_r = (fun (xa, xb) (ya, yb) (za, zb) -> p.assoc_r xa ya za; q.assoc_r xb yb zb);
-  is_unit = (fun (xa, xb) -> p.is_unit xa; q.is_unit xb);
-  refine = (fun (xa, xb) ->
-    (xa, xb) == (p.p.one, q.p.one) \/
-    (p.refine xa /\ q.refine xb /\ ~ (xa == p.p.one) /\ ~ (xb == q.p.one)))
-})
+// val full : pcm' 'a -> 'a -> prop
+// let full #a p x = forall (frame:a{p.composable frame x}). p.op frame x == x
+
+(* This product construction needs some additional assumptions in order to work: *)
+noeq type refined_pcm a = {
+  u: pcm a;
+  (* The unit is the unique "least element" of the preorder defined by
+     [compatible]. (i.e., nothing can be "inside of" or "have less
+     information than" the unit of the PCM) *)
+  compat_unit_unique : x:a ->
+    Lemma (compatible u x u.p.one ==> x == u.p.one);
+// (* refine says that an element is either unit or a full value *)
+// refine_unit_or_full : x:a ->
+//   Lemma (u.refine x == (x == u.p.one \/ full u.p x));
+}
+  
+val tuple_pcm : refined_pcm 'a -> refined_pcm 'b -> refined_pcm ('a & 'b)
+let tuple_pcm #a #b p q =
+  let p' = FStar.PCM.({
+    composable = tuple_comp p.u q.u;
+    op = tuple_op p.u q.u;
+    one = (p.u.p.one, q.u.p.one)
+  }) in
+  let u = FStar.PCM.({
+    p = p';
+    comm = (fun (xa, xb) (ya, yb) -> p.u.comm xa ya; q.u.comm xb yb);
+    assoc = (fun (xa, xb) (ya, yb) (za, zb) -> p.u.assoc xa ya za; q.u.assoc xb yb zb);
+    assoc_r = (fun (xa, xb) (ya, yb) (za, zb) -> p.u.assoc_r xa ya za; q.u.assoc_r xb yb zb);
+    is_unit = (fun (xa, xb) -> p.u.is_unit xa; q.u.is_unit xb);
+    refine = (fun (xa, xb) -> (xa, xb) == p'.one \/ (p.u.refine xa /\ q.u.refine xb))
+  }) in {
+    u = u;
+    compat_unit_unique = (fun (xa, xb) -> p.compat_unit_unique xa; q.compat_unit_unique xb)
+  }
+
+open Steel.Memory
+open Steel.Effect.Atomic
+open Steel.Effect
+
+module T = FStar.Tactics
+
+/// With the alternative definition of frame-preserving updates and
+/// compat_unit_unique, we can define frame-preserving updates for a
+/// tuple PCM from frame-preserving updates on its components:
+
+val compatible_tuple_l :
+  p: refined_pcm 'a -> q: refined_pcm 'b ->
+  x: 'a -> v: 'a -> y: 'b -> w: 'b ->
+  Lemma 
+    (requires compatible p.u x v /\ compatible q.u y w)
+    (ensures compatible (tuple_pcm p q).u (x, y) (v, w))
+let compatible_tuple_l p q x v y w =
+  let pqu = (tuple_pcm p q).u in
+  let aux frame_x frame_y :
+    Lemma 
+      (requires composable pqu (x, y) (frame_x, frame_y) /\
+                op pqu (frame_x, frame_y) (x, y) == (v, w))
+      (ensures compatible pqu (x, y) (v, w))
+      [SMTPat (composable p.u x frame_x); SMTPat (composable q.u y frame_y)] =
+    ()
+  in ()
+
+val upd_fst :
+  p: refined_pcm 'a -> q: refined_pcm 'b ->
+  x: 'a {~ (x == p.u.p.one)} -> y: 'b -> x': 'a ->
+  frame_preserving_upd p.u x x' ->
+  frame_preserving_upd (tuple_pcm p q).u (x, y) (x', y)
+let upd_fst #a #b p q x y x' f (va, vb) =
+  p.compat_unit_unique x;
+  let wa = f va in
+  let pqu = (tuple_pcm p q).u in
+  compatible_tuple_l p q x' wa y vb;
+  let lemma (frame: (a & b) {composable pqu (x, y) frame}):
+    Lemma (composable pqu (x', y) frame /\
+           (op pqu (x, y) frame == (va, vb) ==> op pqu (x', y) frame == (wa, vb)))
+    [SMTPat (composable pqu (x, y) frame)] = ()
+  in (wa, vb)
+
+(*
+val upd_fst_0 :
+  p: refined_pcm 'a -> q: refined_pcm 'b ->
+  r: ref ('a & 'b) (tuple_pcm p q).u ->
+  x: Ghost.erased 'a {~ (Ghost.reveal x == p.u.p.one)} -> y: Ghost.erased 'b -> x': 'a ->
+  frame_preserving_upd p.u x x' ->
+  frame_preserving_upd (tuple_pcm p q).u (Ghost.reveal x, Ghost.reveal y) (x', Ghost.reveal y)
+let upd_fst_0 p q r x y x' upd_x (vx, vy) =
+  assume (compatible (tuple_pcm p q).u (x', Ghost.reveal y) (upd_x vx, vy));
+  // Since x != 1 and compatible x vx, vx != 1 by compat_unit_unique.
+  assert (compatible p.u (Ghost.reveal x) vx);
+  p.compat_unit_unique (Ghost.reveal x);
+  assert (~ (vx == p.u.p.one));
+  // Thus, if refine (vx, vy), vx and vy must be full values.
+  assert ((tuple_pcm p q).u.refine (vx, vy) ==> full (tuple_pcm p q).u.p (vx, vy));
+  full_tup p q vx vy;
+  // A frame-preserving update sends full values to full values, so (upd_x vx, vy) is full too.
+  assume ((tuple_pcm p q).u.refine (vx, vy) ==> full q.u.p vy); (* TODO why doesn't this work? *)
+  assume ((tuple_pcm p q).u.refine (vx, vy) ==> full p.u.p vx); (* TODO why doesn't this work? *)
+  assume (full p.u.p (upd_x vx)); (* can't be unit because upd_x is frame_preserving and vx != unit *)
+  full_tup p q (upd_x vx) vy;
+  assert ((tuple_pcm p q).u.refine (vx, vy) ==> full (tuple_pcm p q).u.p (upd_x vx, vy));
+  assert ((tuple_pcm p q).u.refine (vx, vy) ==> (tuple_pcm p q).u.refine (upd_x vx, vy));
+  assume ((tuple_pcm p q).u.refine (vx, vy) ==> frame_preserving (tuple_pcm p q).u (vx, vy) (upd_x vx, vy));
+  (upd_x vx, vy)
+*)
+
+(*
+val full_tup :
+  p: refined_pcm 'a -> q: refined_pcm 'b -> x: 'a -> y: 'b ->
+  full (tuple_pcm p q).u.p (x, y) == full p.u.p x /\ full q.u.p y
+let full_tup p q x y =
+  (* (forall (x', y') composable with (x, y). (x <> x', y <> y') = (x, y))
+     <=> (forall x' comp w/ x and y' comp w/ y. x <> x' = x /\ y <> y' = y)
+     <=> (forall x' comp w/ x. x <> x' = x) /\ (forall y' comp w/. y <> y' = y) *)
+  admit() (* TODO how to prove this? *)
+  *)
+
+(*
+val frame_preserving_full_value :
+  p: refined_pcm 'a -> x: 'a -> y: 'a ->
+  f:frame_preserving_upd_0 p.u x y ->
+  Lemma (requires full p.u.p x) (ensures full p.u.p (f v))
+let frame_preserving_full_value #a p x y f =
+  compatible_refl p.u x;
+  p.refine_unit_or_full x;
+  assert (p.u.refine x);
+  let z = f x in
+  assert (p.u.refine z);
+  assert (frame_preserving p.u x z);
+  assume (forall (frame:a{composable p.u frame z}). op p.u frame z == z);
+  admit()
+  *)
+
+(*
+val upd_fst_0 :
+  p: refined_pcm 'a -> q: refined_pcm 'b ->
+  r: ref ('a & 'b) (tuple_pcm p q).u ->
+  x: Ghost.erased 'a {~ (Ghost.reveal x == p.u.p.one)} -> y: Ghost.erased 'b -> x': 'a ->
+  frame_preserving_upd_0 p.u x x' ->
+  frame_preserving_upd_0 (tuple_pcm p q).u (Ghost.reveal x, Ghost.reveal y) (x', Ghost.reveal y)
+let upd_fst_0 p q r x y x' upd_x (vx, vy) =
+  assume (compatible (tuple_pcm p q).u (x', Ghost.reveal y) (upd_x vx, vy));
+  // Since x != 1 and compatible x vx, vx != 1 by compat_unit_unique.
+  assert (compatible p.u (Ghost.reveal x) vx);
+  p.compat_unit_unique (Ghost.reveal x);
+  assert (~ (vx == p.u.p.one));
+  // Thus, if refine (vx, vy), vx and vy must be full values.
+  assert ((tuple_pcm p q).u.refine (vx, vy) ==> full (tuple_pcm p q).u.p (vx, vy));
+  full_tup p q vx vy;
+  // A frame-preserving update sends full values to full values, so (upd_x vx, vy) is full too.
+  assume ((tuple_pcm p q).u.refine (vx, vy) ==> full q.u.p vy); (* TODO why doesn't this work? *)
+  assume ((tuple_pcm p q).u.refine (vx, vy) ==> full p.u.p vx); (* TODO why doesn't this work? *)
+  assume (full p.u.p (upd_x vx)); (* can't be unit because upd_x is frame_preserving and vx != unit *)
+  full_tup p q (upd_x vx) vy;
+  assert ((tuple_pcm p q).u.refine (vx, vy) ==> full (tuple_pcm p q).u.p (upd_x vx, vy));
+  assert ((tuple_pcm p q).u.refine (vx, vy) ==> (tuple_pcm p q).u.refine (upd_x vx, vy));
+  assume ((tuple_pcm p q).u.refine (vx, vy) ==> frame_preserving (tuple_pcm p q).u (vx, vy) (upd_x vx, vy));
+  (upd_x vx, vy)
+  *)
+  
+  (*
+  change_slprop (pts_to r (Ghost.reveal x, Ghost.reveal y)) (pts_to r (Ghost.reveal (Ghost.hide (Ghost.reveal x, Ghost.reveal y)))) (fun _ -> ());
+  upd_gen r (Ghost.hide (Ghost.reveal x, Ghost.reveal y)) (Ghost.hide (Ghost.reveal x', Ghost.reveal y)) upd;
+  change_slprop (pts_to r (Ghost.reveal (Ghost.hide (Ghost.reveal x', Ghost.reveal y)))) (pts_to r (Ghost.reveal x', Ghost.reveal y)) (fun _ -> ())*)
 
 /// If no custom PCM is needed, p and q can be instantiated with an all-or-none PCM:
 
@@ -79,7 +294,6 @@ let prod_pcm' #a f p = FStar.PCM.({
   one = prod_one f p;
 })
 
-open FStar.Classical
 val prod_comm :
   f:('a -> Type) -> p:(z:'a -> pcm (f z)) ->
   x:restricted_t 'a f ->
@@ -191,3 +405,125 @@ let union_pcm #a f p = FStar.PCM.({
     | None -> True
     | Some (|xa, xb|) -> (p xa).refine xb /\ ~(xb == (p xa).p.one))
 })
+
+
+(*
+val upd_gen (#a:Type) (#p:pcm a) (r:ref a p) (x y:Ghost.erased a)
+            (f:FStar.PCM.frame_preserving_upd p x y)
+  : SteelT unit
+           (pts_to r x)
+           (fun _ -> pts_to r y)
+           *)
+
+(*
+let upd_first #a #b (r:ref (t a b) pcm_t) (x:Ghost.erased a) (y:a)
+  : SteelT unit (pts_to r (First #a #b x)) (fun _ -> pts_to r (First #a #b y))
+= let f : frame_preserving_upd_0 pcm_t (Ghost.hide (First #a #b x)) (First #a #b y) =
+    fun old_v ->
+      match old_v with
+      | First _ -> First y
+      | Both _ z -> Both y z
+  in
+  change_slprop (pts_to r (First (Ghost.reveal x))) (pts_to r (Ghost.reveal (Ghost.hide (First (Ghost.reveal x))))) (fun _ -> ());
+  upd_gen r (Ghost.hide (First #a #b x)) (Ghost.hide (First #a #b y)) f;
+  change_slprop (pts_to r (Ghost.reveal (Ghost.hide (First y)))) (pts_to r (First y)) (fun _ -> ())
+  *)
+
+(*
+val prod_upd :
+  #a:eqtype -> f:(a -> Type) -> 
+  field:a -> y: f field -> xs: restricted_t a f -> 
+  restricted_t a f
+let prod_upd #a f field y xs =
+  on_domain a (fun field' -> if field = field' then y else xs field')
+
+let frame_preserving_upd #a (p:pcm a) (x y:a) =
+  f: (v:a{compatible p x v}
+      -> Tot (z:a{
+                compatible p y z /\
+                 (p.refine v ==> p.refine z) /\
+                 (p.refine v ==> frame_preserving p v z)}))
+  {
+     forall (v:a{compatible p x v}).
+         let z = f v in
+         (forall (frame:a). {:pattern (composable p v frame)}
+              composable p v frame ==>
+              composable p z frame /\
+              (compatible p x (op p v frame) ==> (op p z frame == f (op p v frame))))
+  }
+
+val frame_preserving_upd_field :
+  #a:eqtype -> f:(a -> Type) -> p:(field:a -> pcm (f field)) ->
+  field:a -> x: f field -> y: f field ->
+  xs: restricted_t a f {xs field == x} ->
+  frame_preserving_upd (p field) x y ->
+  frame_preserving_upd (prod_pcm f p) xs (update f field y xs)
+let frame_preserving_upd_field #a f p field x y xs upd =
+  _
+  *)
+
+(*
+val update : ...
+
+val upd_field :
+  f:('a -> Type) -> p:(z:'a -> pcm (f z)) ->
+  r:ref (restricted_t 'a f) (prod_pcm f p) ->
+  field: 'a -> values: Ghost.erased (restricted_t 'a f{defined only at one field}) ->
+  x: Ghost.erased (f field) -> y: f field ->
+  (frame_preserving_upd_0 (p field) x y) ->
+  SteelT unit (pts_to r (Ghost.reveal values))
+              (fun _ -> pts_to r (update field y values))
+
+let upd_first #a #b (r:ref (t a b) pcm_t) (x:Ghost.erased a) (y:a)
+  : SteelT unit (pts_to r (First #a #b x)) (fun _ -> pts_to r (First #a #b y))
+let f : frame_preserving_upd_0 pcm_t (Ghost.hide (First #a #b x)) (First #a #b y) = fun old_v ->
+    match old_v with
+    | First _ -> First y
+    | Both _ z -> Both y z
+in change_slprop (pts_to r (First (Ghost.reveal x))) (pts_to r (Ghost.reveal (Ghost.hide (First (Ghost.reveal x))))) (fun _ -> ());
+   upd_gen r (Ghost.hide (First #a #b x)) (Ghost.hide (First #a #b y)) f;
+   change_slprop (pts_to r (Ghost.reveal (Ghost.hide (First y)))) (pts_to r (First y)) (fun _ -> ())
+
+
+let upd_first #a #b (r:ref (t a b) pcm_t) (x:Ghost.erased a) (y:a)
+  : SteelT unit (pts_to r (First #a #b x)) (fun _ -> pts_to r (First #a #b y))
+= let f : frame_preserving_upd_0 pcm_t (Ghost.hide (First #a #b x)) (First #a #b y) = fun old_v ->
+    match old_v with
+    | First _ -> First y
+    | Both _ z -> Both y z
+in change_slprop (pts_to r (First (Ghost.reveal x))) (pts_to r (Ghost.reveal (Ghost.hide (First (Ghost.reveal x))))) (fun _ -> ());
+   upd_gen r (Ghost.hide (First #a #b x)) (Ghost.hide (First #a #b y)) f;
+   change_slprop (pts_to r (Ghost.reveal (Ghost.hide (First y)))) (pts_to r (First y)) (fun _ -> ())
+
+
+let upd_first #a #b (r:ref (t a b) pcm_t) (x:Ghost.erased a) (y:a)
+  : SteelT unit (pts_to r (First #a #b x)) (fun _ -> pts_to r (First #a #b y))
+= let f : frame_preserving_upd_0 pcm_t (Ghost.hide (First #a #b x)) (First #a #b y) = fun old_v ->
+    match old_v with
+    | First _ -> First y
+    | Both _ z -> Both y z
+in change_slprop (pts_to r (First (Ghost.reveal x))) (pts_to r (Ghost.reveal (Ghost.hide (First (Ghost.reveal x))))) (fun _ -> ());
+   upd_gen r (Ghost.hide (First #a #b x)) (Ghost.hide (First #a #b y)) f;
+   change_slprop (pts_to r (Ghost.reveal (Ghost.hide (First y)))) (pts_to r (First y)) (fun _ -> ())
+
+
+// TODO frame-preserving updates
+// move 2d point along x
+// move 2d point along y
+// given a function "incrementX" and "incrementY"; write a function that calls it in a loop
+
+// union examples
+// 2d & 3d point
+// rgb / hsv
+
+// next examples:
+//   swap 2 3d points with a helper function
+//   union where discrimnant is not just a tag, but some predicate
+
+// { f field_x = Full .. }
+// { p `pts_to` f } 
+//   addr_of p field_x
+// { fun q -> (p `pts_to` f \ x) `star` (q `pts_to` x) }
+// 
+// let q = addr_of p field_x
+*)
